%

\documentclass{article}
\usepackage{amsmath}
\begin{document}

\section{Problem A}
\subsection{Analytical Solution}
\begin{align}
cov(X_n,X_{n+1})=E[X_nX_{n+1}]-EX_nEX_{n+1} \\
E[X_nX_{n+1}]=\sum_{i=0}^{\infty}E[X_nX_{n+1}|X_n=i]P(X_n=i) \\
=\sum_{i=0}^{\infty}iE[X_{n+1}|X_n=i]P(X_n=i) \notag\\
=\sum_{i=0}^{\infty}i(E[X_n|X_n=i]+E[I_n|X_n=i])P(X_n=i) \notag\\
=\sum_{i=0}^{\infty}i(i+E[I_n|X_n=i])P(X_n=i) \notag\\
=\sum_{i=0}^{\infty}i(i+(\alpha_i-\beta_i))P(X_n=i) \notag\\
EX_n=\sum_{i=0}^{\infty}iP(X_n=i) \\
EX_{n+1}=EX_n+EI_n \\
=EX_n+\sum_{i=0}^{\infty}E[I_n|X_n=i]P(X_n=i) \notag\\
=EX_n+\sum_{i=0}^{\infty}(\alpha_i-\beta_i)P(X_n=i) \notag\\
\text{From (1), }(2)-(3)*(4)\Rightarrow \notag\\
\lim_{n\rightarrow\infty}cov(X_n,X_{n+1})=\sum_{i=0}^{\infty}i(i+\alpha_i-\beta_i)\pi_i-\sum_{i=0}^{\infty}i\pi_i\sum_{i=0}^{\infty}(i+\alpha_i-\beta_i)\pi_i
\end{align}
\subsection{Simulation Results}
(todo)
\end{document}

